%! Author = herbertxin

\documentclass[twocolumn, fleqn]{article}
\usepackage[margin=1in]{geometry}
\usepackage{fancyhdr}
\usepackage{graphicx}
\usepackage{amsmath}
\usepackage{hyperref}
\usepackage{enumitem}
\usepackage{amssymb}
\usepackage{tcolorbox}



% Adjust column separation and add vertical rule
\setlength{\columnsep}{25pt} % Increase space between columns
\setlength{\columnseprule}{0.6pt}
\setlength{\jot}{6pt} % Set the space between equation lines to 6pt
\setlength{\parskip}{3pt}

% Header and Footer Settings
\pagestyle{fancy}
\fancyhf{}
\lhead{Course}
\chead{Real Business Cycle}
\rhead{Page \thepage}
\renewcommand{\headrulewidth}{0.4pt}
\newtcolorbox{note}[1][]{
	enhanced,
	colback=white,            % Background color of the box content
	colframe=black,           % Border color
	coltitle=white,           % Title text color
	colbacktitle=black,       % Background color of the title area
	fonttitle=\bfseries,      % Bold font for the title
	boxrule=1pt,              % Border thickness
	title=SIDENOTE,           % Title of the box
	sharp corners,            % Square corners
	before skip=10pt,         % Space before the box
	after skip=10pt,          % Space after the box
	left=5pt,                 % Left padding
	right=5pt,                % Right padding
	top=5pt,                  % Top padding
	bottom=5pt,               % Bottom padding
	width=\columnwidth,       % Box width matches column width
	#1                        % Allows for optional parameters
}

\begin{document}

	\title{Real Business Cycle}
	\author{Herbert W. Xin}
	\date{\today}
	\maketitle

	\tableofcontents
	\thispagestyle{fancy}
	
	\section{Hodrick-Prescott Filter}
	
	In analyzing real world datas, it is often useful to separate the trend data from business cycle variation. In essence, we want 
	\[\ln(Y_t) = \ln (Y_t^{\text{trend}})+\ln (Y_t^{\text{cycle}})\]
	
	To simplify the expression, we can rewrite this as 
	\[y_t = y_t^{\text{trend}}+y_t^\text{cycle}\]
	
	Now, the HP-filter makes the decomposition by solving the minimization problem of 
	\begin{align*}
		&\min_{y_t^{\text{trend}}}\sum_{t=1}^{T} (y_t-y_t^{\text{trend}})^2 \\
		&+\lambda \sum_{t=1}^{T} \left[ (y_{t+1}^{\text{trend}}- y_{t}^{\text{trend}})-(y_{t}^{\text{trend}}-y_{t-1}^{\text{trend}})\right]^2
	\end{align*}
	subject to 
	\[y_t = y_t^{\text{trend}}+y_t^\text{cycle}\]
	
	The first term measures the difference between trend and the actual data, while the second term measures the difference between changes in trend.
	
	Thus, the parameter $\lambda$ measures the trade off between fit of the data and movement in trends. The higher the $\lambda$, the more weight we put on the smoothness of the trend. 
	
	If $\lambda=0$ then all the weight are put on the first term, so to minimize the difference we would just set trend equals to $y_t$
	
	\section{The Model}
	\subsection{Households}
	Household solves the utility maximization problem of 
	\begin{align*}
		\max_{c_t} u(c_t) &= \sum_{t=0}^{T} \beta^t U(c_t)
	\end{align*}
	subject to 
	\begin{align*}
	c_t + a_{t+1} &= w_t + (1 + r_t) a_t \\
	c_t &\geq 0 \\
	a_{T+1} &= 0
	\end{align*}
	
	The usual Inada conditions and restriction applies here.
	
	Set up the Lagrangian gives 
	\[
	L = \sum_{t=0}^T \beta^t U(c_t) + \sum_{t=0}^T \lambda_t \big(w_t + (1 + r_t)a_t - c_t - a_{t+1}\big)
	\]
	Solving for FOCs give
	\begin{align*}
	\beta^t U'(c_t) &= \lambda_t \\
	\beta^{t+1} U'(c_{t+1}) &= \lambda_{t+1} \\
	\lambda_t &= \lambda_{t+1} (1 + r_{t+1}) \\
	U'(c_t) &= \beta (1 + r_{t+1}) U'(c_{t+1})
	\end{align*}
	where the last equation is our familiar Euler equation.
	
	In steady state, we have
	\[1 = \beta (1+r)\]
	
	Using the budget constraint
	\begin{align*}
	c_t &= w_t + (1 + r_t)a_t - a_{t+1} \\
	c_{t+1} &= w_{t+1} + (1 + r_{t+1})a_{t+1} - a_{t+2} 
	\end{align*}
	
	We can rewrite the Euler equation as 
	\begin{align*}
			&U'(w_t + (1 + r_t)a_t - a_{t+1}) \\
			&= \beta (1 + r_{t+1}) U'(w_{t+1} + (1 + r_{t+1})a_{t+1} - a_{t+2})
	\end{align*}
	
	\subsection{Firms}
	The production technology is standard neoclassical Cobb-Douglas production function
	\[y_t = A_t k_t^\alpha n_t^{\alpha-1}\]
	For now, we assume $A_t =A$
	\[y_t = A k_t^\alpha n_t^{\alpha-1}\]
	
	We denote the rental price per unit of capital as $\mu_t$, so the return rate is 
	\[r_t = \mu_t -\delta\]
	
	Then the firms solves the profit maximization problem
	\begin{align*}
		\max_{n_t, k_t} (y_t - w_t n_t -\mu_t k_t)
	\end{align*}
	subject to 
	\begin{align*}
		y_t &= Ak_t^\alpha n_t^{1-\alpha}\\
		&k_t, n_t \geq 0
	\end{align*}
	
	The FOC yields 
	\begin{align*}
		w_t &= (1 - \alpha)A \left(\frac{k_t}{n_t}\right)^\alpha \\
		\mu_t &= \alpha A \left(\frac{k_t}{n_t}\right)^{\alpha-1} 
	\end{align*}
	
	So the profit function becomes 
	\begin{align*}
		\pi_t &= Ak_t^\alpha n_t^{1-\alpha} - w_t n_t - \mu_t k_t \\
	&= Ak_t^\alpha n_t^{1-\alpha} - (1 - \alpha)A \left(\frac{k_t}{n_t}\right)^\alpha n_t \\
	&- \alpha A \left(\frac{k_t}{n_t}\right)^{\alpha-1} k_t = 0
	\end{align*}
	
	\subsection{Competitive Equilibrium}
	Since the economy resource constraint is 
	\begin{align*}
		y_t &= c_t + I_t\\
		I_t &= k_{t+1} - (1-\delta)k_t\\
		c_t &+ k_{t+1} - (1-\delta)k_t = Ak_t^\alpha n_t^{1-\alpha}
	\end{align*}
	The last equation is then the exact market clearing condition. We would also have $n_t=1, a_t = k_t$.
	
	Since we know the wage and capital return from the firm's profit maximization problem, we can substitute those into the Euler's equation, which gives
	\begin{align*}
	&U'\big((1 - \alpha)A k_t^\alpha + (1 + \alpha A(k_t)^{\alpha-1} - \delta)k_t - k_{t+1}\big) \\
	&= \beta (1 + \alpha A(k_{t+1})^{\alpha-1} - \delta) A(k_{t+1})^{\alpha-1} - \delta)k_{t+1}\\& - k_{t+2}\big) \\[10pt]
	&U'(A k_t^\alpha + (1 - \delta)k_t - k_{t+1}) 
	= \beta (1 + \alpha A(k_{t+1})^{\alpha-1} - \delta) \\
	&\quad \cdot U'(A k_{t+1}^\alpha + (1 - \delta)k_{t+1} - k_{t+2})
	\end{align*}
	
	Given the boundary condition $k_0 = a_0, \text{ and } k_{T+1}=a_{T+1} = 0$, we can solve for the problem.
	
	\subsection{Social Planner Problem}
	The social planner solves the problem of 
	\begin{align*}
	\max_{\{c_t, k_{t+1}\}_{t=0}^T} &\sum_{t=0}^T \beta^t U(c_t) \\
	&\text{s.t.} \quad c_t + k_{t+1} - (1 - \delta)k_t = A k_t^\alpha \\
	c_t &\geq 0, \quad k_0 > 0 \, \text{given}
	\end{align*}
	
	Set up the Lagrangian and solve for the FOC gives
	\begin{align*}
	L &= \sum_{t=0}^T \beta^t U(c_t) + \sum_{t=0}^T \lambda_t \big[A k_t^\alpha - c_t - k_{t+1} + (1 - \delta)k_t\big] \\
	\frac{\partial L}{\partial c_t} &= \beta^t U'(c_t) - \lambda_t = 0 \\
	\frac{\partial L}{\partial c_{t+1}} &= \beta^{t+1} U'(c_{t+1}) - \lambda_{t+1} = 0 \\
	\frac{\partial L}{\partial k_{t+1}} &= -\lambda_t + \lambda_{t+1} \big[\alpha A k_{t+1}^{\alpha - 1} + (1 - \delta)\big] = 0
	\end{align*}
	
	
	Combining the FOCs give the Euler equation
	\begin{align*}
	\beta^t U'(c_t) &= \lambda_t = \lambda_{t+1} \big[\alpha A k_{t+1}^{\alpha - 1} + (1 - \delta)\big] \\
	&= \beta^{t+1} U'(c_{t+1}) \big[\alpha A k_{t+1}^{\alpha - 1} + (1 - \delta)\big] \\[5pt]
	U'(c_t) &= \beta U'(c_{t+1}) \big[\alpha A k_{t+1}^{\alpha - 1} + (1 - \delta)\big]
	\end{align*}
	
	Using the resource constraints 
	\begin{align*}
	c_t &= A k_t^\alpha - k_{t+1} + (1 - \delta)k_t \\
	c_{t+1} &= A k_{t+1}^\alpha - k_{t+2} + (1 - \delta)k_{t+1} \\
	U'(A k_t^\alpha - &k_{t+1} + (1 - \delta)k_t) = \beta U'(A k_{t+1}^\alpha - k_{t+2} +\\& (1 - \delta)k_{t+1}) \cdot \big[\alpha A k_{t+1}^{\alpha - 1} + (1 - \delta)\big]
	\end{align*}
	
	which is exactly the same as the Euler equation from the competitive equilibrium.
	
	\subsection{Steady State}
	In steady state, we set $c_{t} = c_{t+1} = c^\ast$ and $k_t = k_{t+1} =k^\ast$, which changes the Euler equation to 
	\[
	1 = \beta \big[\alpha A (k^*)^{\alpha - 1} + (1 - \delta)\big]
	\]
	
	Solving for $k^\ast$ gives
	\[
	k^* = \left[\frac{\alpha A \beta}{1 - (1 - \delta)\beta}	\right]^{\frac{1}{1 - \alpha}}
	\]
	
	and the steady state consumption is 
	\[ c^\ast = A(k^\ast)^\alpha - \delta k^\ast\]
	
	\section{Dynamic Analysis}
	
	Since we have the Euler equation
	\begin{align*}
		&U'(A k_t^\alpha + (1 - \delta)k_t - k_{t+1}) 
	= \beta (1 + \\
	&\alpha A(k_{t+1})^{\alpha-1} - \delta) 
	U'(A k_{t+1}^\alpha + (1 - \delta)k_{t+1} - k_{t+2})
	\end{align*}
	
	
	
	
	
	
	
	
\end{document}